confluence proof of the System F

coq/LC/Debruijn/F.v
@@ -48,6 +48,15 @@ Fixpoint subst_typ n ts t :=
     | tyabs t => tyabs (subst_typ n.+1 ts t)
   end.
 
+Fixpoint typemap (f : nat -> typ -> typ) n t :=
+  match t with
+    | var m => var m
+    | app tl tr => app (typemap f n tl) (typemap f n tr)
+    | abs ty t => abs (f n ty) (typemap f n t)
+    | uapp t ty => uapp (typemap f n t) (f n ty)
+    | uabs t => uabs (typemap f n.+1 t)
+  end.
+
 Fixpoint shift_term d c t :=
   match t with
     | var n => var (if c <= n then n + d else n)
@@ -57,57 +66,21 @@ Fixpoint shift_term d c t :=
     | uabs t => uabs (shift_term d c t)
   end.
 
-Definition subst_termv ts m n :=
-  shift_term n 0 (nth (var (m - n - size ts)) ts (m - n)).
+Definition subst_termv ts m n n' :=
+  typemap (shift_typ n') 0
+    (shift_term n 0
+      (nth (var (m - n - size ts)) ts (m - n))).
 
-Fixpoint subst_term n ts t :=
+Fixpoint subst_term n n' ts t :=
   match t with
-    | var m => if n <= m then subst_termv ts m n else m
-    | app tl tr => app (subst_term n ts tl) (subst_term n ts tr)
-    | abs ty t => abs ty (subst_term n.+1 ts t)
-    | uapp t ty => uapp (subst_term n ts t) ty
-    | uabs t => uabs (subst_term n ts t)
-  end.
-
-Fixpoint type_map (f : nat -> typ -> typ) n t :=
-  match t with
-    | var m => var m
-    | app tl tr => app (type_map f n tl) (type_map f n tr)
-    | abs ty t => abs (f n ty) (type_map f n t)
-    | uapp t ty => uapp (type_map f n t) (f n ty)
-    | uabs t => uabs (type_map f n.+1 t)
+    | var m => if n <= m then subst_termv ts m n n' else m
+    | app tl tr => app (subst_term n n' ts tl) (subst_term n n' ts tr)
+    | abs ty t => abs ty (subst_term n.+1 n' ts t)
+    | uapp t ty => uapp (subst_term n n' ts t) ty
+    | uabs t => uabs (subst_term n n'.+1 ts t)
   end.
 
 Definition shift_context d c ctx := map (Option.map (shift_typ d c)) ctx.
-
-Reserved Notation "t ->r1 t'" (at level 70, no associativity).
-Reserved Notation "t ->rp t'" (at level 70, no associativity).
-
-Inductive reduction1 : relation term :=
-  | red1fst  : forall ty t1 t2, app (abs ty t1) t2 ->r1 subst_term 0 [:: t2] t1
-  | red1snd  : forall t ty,
-               uapp (uabs t) ty ->r1 type_map (subst_typ^~ [:: ty]) 0 t
-  | red1appl : forall t1 t1' t2, t1 ->r1 t1' -> app t1 t2 ->r1 app t1' t2
-  | red1appr : forall t1 t2 t2', t2 ->r1 t2' -> app t1 t2 ->r1 app t1 t2'
-  | red1abs  : forall ty t t', t ->r1 t' -> abs ty t ->r1 abs ty t'
-  | red1uapp : forall t t' ty, t ->r1 t' -> uapp t ty ->r1 uapp t' ty
-  | red1uabs : forall t t', t ->r1 t' -> uabs t ->r1 uabs t'
-  where "t ->r1 t'" := (reduction1 t t').
-
-Notation reduction := [* reduction1].
-Infix "->r" := reduction (at level 70, no associativity).
-
-Inductive parred : relation term :=
-  | parredfst  : forall ty t1 t1' t2 t2', t1 ->rp t1' -> t2 ->rp t2' ->
-                 app (abs ty t1) t2 ->rp subst_term 0 [:: t2'] t2'
-  | parredsnd  : forall t t' ty, t ->rp t' ->
-                 uapp (uabs t) ty ->rp type_map (subst_typ^~ [:: ty]) 0 t'
-  | parredapp  : forall t1 t1' t2 t2',
-                 t1 ->rp t1' -> t2 ->rp t2' -> app t1 t2 ->rp app t1' t2'
-  | parredabs  : forall ty t t', t ->rp t' -> abs ty t ->rp abs ty t'
-  | parreduapp : forall t t' ty, t ->rp t' -> uapp t ty ->rp uapp t' ty
-  | parreduabs : forall t t', t ->rp t' -> uabs t ->rp uabs t'
-  where "t ->rp t'" := (parred t t').
 
 Inductive typing : context typ -> term -> typ -> Prop :=
   | typvar  : forall ctx n ty, ctxindex ctx n ty -> typing ctx (var n) ty
@@ -124,6 +97,23 @@ Inductive typing : context typ -> term -> typ -> Prop :=
               typing (shift_context 1 0 ctx) t ty ->
               typing ctx (uabs t) (tyabs ty).
 
+Reserved Notation "t ->r1 t'" (at level 70, no associativity).
+
+Inductive reduction1 : relation term :=
+  | red1fst  : forall ty t1 t2,
+               app (abs ty t1) t2 ->r1 subst_term 0 0 [:: t2] t1
+  | red1snd  : forall t ty,
+               uapp (uabs t) ty ->r1 typemap (subst_typ^~ [:: ty]) 0 t
+  | red1appl : forall t1 t1' t2, t1 ->r1 t1' -> app t1 t2 ->r1 app t1' t2
+  | red1appr : forall t1 t2 t2', t2 ->r1 t2' -> app t1 t2 ->r1 app t1 t2'
+  | red1abs  : forall ty t t', t ->r1 t' -> abs ty t ->r1 abs ty t'
+  | red1uapp : forall t t' ty, t ->r1 t' -> uapp t ty ->r1 uapp t' ty
+  | red1uabs : forall t t', t ->r1 t' -> uabs t ->r1 uabs t'
+  where "t ->r1 t'" := (reduction1 t t').
+
+Notation reduction := [* reduction1].
+Infix "->r" := reduction (at level 70, no associativity).
+
 Lemma shiftzero_ty : forall n t, shift_typ 0 n t = t.
 Proof.
   move => n t; elim: t n => /=; try congruence.
@@ -131,12 +121,12 @@ Proof.
 Qed.
 
 Lemma shift_add_ty :
-  forall d d' c c' t, c <= c' <= d + c ->
+  forall d c d' c' t, c <= c' <= d + c ->
   shift_typ d' c' (shift_typ d c t) = shift_typ (d' + d) c t.
 Proof.
-  move => d d' c c' t; elim: t c c' => /=.
+  move => d c d' c' t; elim: t c c' => /=.
   - move => n c c' H; elimif_omega.
-  - move => t1 ? t2 ? c c' ?; f_equal; auto.
+  - by move => tl IHtl tr IHtr c c' ?; rewrite IHtl // IHtr.
   - by move => t IH c c' ?; rewrite IH // addnS !ltnS.
 Qed.
 
@@ -147,8 +137,19 @@ Lemma shift_shift_distr_ty :
 Proof.
   move => d c d' c' t; elim: t c c' => /=.
   - move => n c c' ?; elimif_omega.
-  - move => t1 ? t2 ? c c' ?; f_equal; auto.
+  - by move => tl IHtl tr IHtr c c' ?; rewrite IHtl // IHtr.
   - by move => t' IH c c' ?; rewrite -addnS IH.
+Qed.
+
+Lemma shift_subst_distr_ty :
+  forall n d c ts t, c <= n ->
+  shift_typ d c (subst_typ n ts t) = subst_typ (d + n) ts (shift_typ d c t).
+Proof.
+  move => n d c ts t; elim: t n c => /=.
+  - move => n m c H; elimif_omega.
+    by rewrite /subst_typv shift_add_ty ?addn0 // (addnC n) subnDl.
+  - by move => tl IHtl tr IHtr n c H; rewrite IHtl // IHtr.
+  - by move => t IH n c H; rewrite -addnS IH.
 Qed.
 
 Lemma subst_shift_distr_ty :
@@ -156,72 +157,204 @@ Lemma subst_shift_distr_ty :
   shift_typ d (n + c) (subst_typ n ts t) =
   subst_typ n (map (shift_typ d c) ts) (shift_typ d (size ts + n + c) t).
 Proof.
-  move => n d c ts t; elim: t n => /=.
-  - move => m n; rewrite /subst_typv size_map; elimif_omega.
-    - rewrite !nth_default ?size_map /=; try ssromega.
-      rewrite (subnAC _ n) subnK; elimif_omega.
-    - rewrite -shift_shift_distr_ty // nth_map' /=.
-      f_equal; apply nth_equal; rewrite size_map; elimif_omega.
-  - congruence.
-  - by move => t IH n; rewrite (IH n.+1) addnS addSn.
-Qed.
-
-Lemma shift_subst_distr_ty :
-  forall n d c t ts, c <= n ->
-  shift_typ d c (subst_typ n ts t) = subst_typ (d + n) ts (shift_typ d c t).
-Proof.
-  move => n d c t ts; elim: t n c => /=.
-  - move => n m c H; elimif_omega.
-    by rewrite /subst_typv shift_add_ty ?addn0 // (addnC n) subnDl.
-  - move => tl IHl tr IHr n c H; f_equal; auto.
-  - move => t IH n c H; f_equal; rewrite -addnS IH //.
+  move => n d c ts t; elim: t n => /=; try (move: addnS addSn; congruence).
+  move => m n; rewrite /subst_typv size_map; elimif_omega.
+  - rewrite !nth_default ?size_map /=; try ssromega.
+    rewrite (subnAC _ n) subnK; elimif_omega.
+  - rewrite -shift_shift_distr_ty // nth_map' /=.
+    f_equal; apply nth_equal; rewrite size_map; elimif_omega.
 Qed.
 
 Lemma subst_shift_cancel_ty :
-  forall n d c t ts, n <= d ->
-  subst_typ (c + n) ts (shift_typ (size ts + d) c t) = shift_typ d c t.
+  forall n d c ts t, c <= n -> size ts <= d -> n - c <= d - size ts ->
+  subst_typ n ts (shift_typ d c t) = shift_typ (d - size ts) c t.
 Proof.
-  move => n d c t ts; elim: t c => /=.
-  - move => v c H; elimif_omega.
+  move => n d c ts t; elim: t n c => /=.
+  - move => v n c H H0 H1; elimif_omega.
     rewrite /subst_typv nth_default /=; f_equal; ssromega.
-  - by move => tl IHtl tr IHtr c H; rewrite IHtl // IHtr.
-  - by move => t IH c H; rewrite -addSn IH.
+  - by move => tl IHtl tr IHtr n c H H0 H1; rewrite IHtl // IHtr.
+  - by move => t IH n c H H0 H1; rewrite IH.
 Qed.
 
 Lemma subst_subst_distr_ty :
-  forall n m t xs ys,
+  forall n m xs ys t,
   subst_typ (m + n) xs (subst_typ m ys t) =
   subst_typ m (map (subst_typ n xs) ys) (subst_typ (size ys + m + n) xs t).
 Proof.
-  move => n m t; elim: t m => /=.
-  - move => v m xs ys; elimif_omega; rewrite /subst_typv.
-    - rewrite -{5}(add0n m) -addnA -{2}(size_map (subst_typ n xs) ys)
-        subst_shift_cancel_ty; last apply leq_addr.
-      rewrite nth_default /=; last ssromega.
-      rewrite /subst_typv subnAC subnK ?subnDA; elimif_omega.
-    - rewrite -shift_subst_distr_ty // size_map nth_map'; f_equal.
-      apply nth_equal; rewrite size_map /=; elimif_omega.
-  - congruence.
-  - by move => t IH m xs ys; rewrite -addSn IH addnS addSn.
+  move => n m xs ys t; elim: t m => /=; try (move: addnS addSn; congruence).
+  move => v m; elimif_omega; rewrite /subst_typv.
+  - rewrite (subst_shift_cancel_ty m) // size_map; try ssromega.
+    rewrite -{1}addnA addKn nth_default /=; last ssromega.
+    rewrite /subst_typv subnAC subnK ?subnDA; elimif_omega.
+  - rewrite -shift_subst_distr_ty // size_map nth_map'; f_equal.
+    apply nth_equal; rewrite size_map /=; elimif_omega.
 Qed.
 
 Lemma subst_app_ty :
-  forall n t xs ys,
+  forall n xs ys t,
   subst_typ n xs (subst_typ (size xs + n) ys t) = subst_typ n (xs ++ ys) t.
 Proof.
-  move => n t xs ys; elim: t n => /=.
-  - move => v n; elimif_omega; rewrite /subst_typv.
-    - rewrite -{1}(add0n n) subst_shift_cancel_ty //
-        nth_cat size_cat !subnDA (subnAC _ (size xs)); f_equal; elimif_omega.
-    - rewrite nth_cat; f_equal; elimif_omega; apply nth_equal; ssromega.
-  - congruence.
-  - by move => t IH n; rewrite -addnS IH.
+  move => n xs ys t; elim: t n => /=; try (move: addnS; congruence).
+  move => v n; elimif_omega; rewrite /subst_typv.
+  - rewrite subst_shift_cancel_ty; try ssromega.
+    rewrite size_cat nth_cat !subnDA addKn (subnAC _ (size xs)); elimif_omega.
+  - rewrite nth_cat; f_equal; elimif_omega; apply nth_equal; ssromega.
 Qed.
 
 Lemma subst_nil_ty : forall n t, subst_typ n [::] t = t.
 Proof.
   move => n t; elim: t n => /=; try congruence.
   move => v n; rewrite /subst_typv nth_nil /= -fun_if; elimif_omega.
+Qed.
+
+Lemma typemap_compose :
+  forall f g n m t,
+  typemap f n (typemap g m t) =
+  typemap (fun i ty => f (i + n) (g (i + m) ty)) 0 t.
+Proof.
+  move => f g n m t; elim: t n m => //=.
+  - by move => tl IHtl tr IHtr n m; rewrite IHtl IHtr.
+  - by move => ty t IH n m; rewrite IH.
+  - by move => t IH ty n m; rewrite IH.
+  - move => t IH n m; rewrite {}IH; f_equal.
+    elim: t (0) => //=; move: addSnnS; congruence.
+Qed.
+
+Lemma typemap_eq' :
+  forall f g n m t,
+  (forall o t, f (o + n) t = g (o + m) t) -> typemap f n t = typemap g m t.
+Proof.
+  move => f g n m t H; elim: t n m H => //=.
+  - move => tl IHtl tr IHtr n m H; f_equal; auto.
+  - move => ty t IH n m H; f_equal; auto.
+    rewrite -(add0n n) -(add0n m); auto.
+  - move => t IH ty n m H; f_equal; auto.
+    rewrite -(add0n n) -(add0n m); auto.
+  - move => t IH n m H; f_equal; apply IH => o ty.
+    by rewrite -!addSnnS.
+Qed.
+
+Lemma typemap_eq :
+  forall f g n t, (forall n t, f n t = g n t) -> typemap f n t = typemap g n t.
+Proof.
+  move => f g n t H; apply typemap_eq' => {t} o; apply H.
+Qed.
+
+Lemma shifttyp_add :
+  forall d c d' c' t, c <= c' <= d + c ->
+  typemap (shift_typ d') c' (typemap (shift_typ d) c t) =
+  typemap (shift_typ (d' + d)) c t.
+Proof.
+  move => d c d' c' t H.
+  rewrite typemap_compose. apply typemap_eq' => {t} n t.
+  by rewrite addn0 shift_add_ty // addnCA !leq_add2l.
+Qed.
+
+Lemma shifttyp_shifttyp_distr :
+  forall d c d' c' t, c' <= c ->
+  typemap (shift_typ d') c' (typemap (shift_typ d) c t) =
+  typemap (shift_typ d) (d' + c) (typemap (shift_typ d') c' t).
+Proof.
+  move => d c d' c' t H.
+  rewrite !typemap_compose; apply typemap_eq => {t} n t.
+  rewrite shift_shift_distr_ty; f_equal; ssromega.
+Qed.
+
+Lemma shifttyp_substtyp_distr :
+  forall n d c ts t, c <= n ->
+  typemap (shift_typ d) c (typemap (subst_typ^~ ts) n t) =
+  typemap (subst_typ^~ ts) (d + n) (typemap (shift_typ d) c t).
+Proof.
+  move => n d c ts t H.
+  rewrite !typemap_compose; apply typemap_eq => {t} n' t.
+  rewrite shift_subst_distr_ty; f_equal; ssromega.
+Qed.
+
+Lemma substtyp_shifttyp_distr :
+  forall n d c ts t,
+  typemap (shift_typ d) (n + c) (typemap (subst_typ^~ ts) n t) =
+  typemap (subst_typ^~ (map (shift_typ d c) ts)) n
+    (typemap (shift_typ d) (size ts + n + c) t).
+Proof.
+  move => n d c ts t.
+  rewrite !typemap_compose; apply typemap_eq => {t} n' t.
+  by rewrite addnA subst_shift_distr_ty !addnA (addnC (size _)).
+Qed.
+
+Lemma substtyp_substtyp_distr :
+  forall n m xs ys t,
+  typemap (subst_typ^~ xs) (m + n) (typemap (subst_typ^~ ys) m t) =
+  typemap (subst_typ^~ (map (subst_typ n xs) ys)) m
+    (typemap (subst_typ^~ xs) (size ys + m + n) t).
+Proof.
+  move => n m xs ys t.
+  rewrite !typemap_compose; apply typemap_eq => {t} n' t.
+  by rewrite addnA subst_subst_distr_ty !addnA (addnC (size _)).
+Qed.
+
+Lemma shift_typemap_distr :
+  forall f d c n t,
+  shift_term d c (typemap f n t) = typemap f n (shift_term d c t).
+Proof.
+  move => f d c n t; elim: t d c n => /=; congruence.
+Qed.
+
+Lemma subst_shifttyp_distr :
+  forall n m d c ts t, c <= m ->
+  subst_term n (d + m) ts (typemap (shift_typ d) c t) =
+  typemap (shift_typ d) c (subst_term n m ts t).
+Proof.
+  move => n m d c ts t; elim: t n m c => /=.
+  - move => v n m c H; rewrite /subst_termv; elimif_omega.
+    by rewrite -!shift_typemap_distr shifttyp_add // addn0.
+  - by move => tl IHtl tr IHtr n m c H; rewrite IHtl // IHtr.
+  - by move => ty t IH n m c H; rewrite IH.
+  - by move => t IH ty n m c H; rewrite IH.
+  - by move => t IH n m c H; rewrite -addnS IH.
+Qed.
+
+Lemma shifttyp_subst_distr :
+  forall d c n m ts t,
+  typemap (shift_typ d) (m + c) (subst_term n m ts t) =
+  subst_term n m (map (typemap (shift_typ d) c) ts)
+    (typemap (shift_typ d) (m + c) t).
+Proof.
+  move => d c n m ts t; elim: t n m => /=; try (move: addSn; congruence).
+  move => v n m; elimif_omega.
+  by rewrite /subst_termv size_map -!shift_typemap_distr
+    -shifttyp_shifttyp_distr // (nth_map' (typemap _ _)).
+Qed.
+
+Lemma subst_substtyp_distr :
+  forall n m m' tys ts t, m' <= m ->
+  subst_term n m ts (typemap (subst_typ^~ tys) m' t) =
+  typemap (subst_typ^~ tys) m' (subst_term n (size tys + m) ts t).
+Proof.
+  move => n m m' tys ts t; elim: t n m m' => /=.
+  - move => v n m m' H; elimif_omega.
+    rewrite /subst_termv -!shift_typemap_distr typemap_compose.
+    f_equal; apply typemap_eq => {v n ts H0} n t.
+    by rewrite addn0 subst_shift_cancel_ty ?addKn // leq_addr.
+  - by move => tl IHtl tr IHtr n m m' H; rewrite IHtl // IHtr.
+  - by move => ty t IH n m m' H; rewrite IH.
+  - by move => t IH ty n m m' H; rewrite IH.
+  - by move => t IH n m m' H; rewrite IH // addnS.
+Qed.
+
+Lemma substtyp_subst_distr :
+  forall n m m' tys ts t, m <= m' ->
+  typemap (subst_typ^~ tys) m' (subst_term n m ts t) =
+  subst_term n m (map (typemap (subst_typ^~ tys) (m' - m)) ts)
+    (typemap (subst_typ^~ tys) m' t).
+Proof.
+  move => n m m' tys ts t; elim: t n m m' => /=.
+  - move => v n m m' H; elimif_omega.
+    by rewrite /subst_termv size_map -!shift_typemap_distr
+      -{1}(subnKC H) -shifttyp_substtyp_distr // (nth_map' (typemap _ _)) /=.
+  - by move => tl IHtl tr IHtr n m m' H; rewrite IHtl // IHtr.
+  - by move => ty t IH n m m' H; rewrite IH.
+  - by move => t IH ty n m m' H; rewrite IH.
+  - by move => t IH n m m' H; rewrite IH.
 Qed.
 
 Lemma shiftzero : forall n t, shift_term 0 n t = t.
@@ -231,13 +364,13 @@ Proof.
 Qed.
 
 Lemma shift_add :
-  forall d d' c c' t, c <= c' <= d + c ->
+  forall d c d' c' t, c <= c' <= d + c ->
   shift_term d' c' (shift_term d c t) = shift_term (d' + d) c t.
 Proof.
-  move => d d' c c' t; elim: t c c' => /=.
+  move => d c d' c' t; elim: t c c' => /=.
   - move => n c c' H; elimif_omega.
-  - move => t1 ? t2 ? c c' ?; f_equal; auto.
-  - by move => ty t IH c c' ?; rewrite IH // addnS !ltnS.
+  - move => t1 H t2 H0 c c' H1; f_equal; auto.
+  - by move => ty t IH c c' H; rewrite IH // addnS !ltnS.
   - by move => t IH ty c c' H; rewrite IH.
   - by move => t IH c c' H; rewrite IH.
 Qed.
@@ -248,83 +381,257 @@ Lemma shift_shift_distr :
   shift_term d (d' + c) (shift_term d' c' t).
 Proof.
   move => d c d' c' t; elim: t c c' => /=.
-  - move => n c c' ?; elimif_omega.
-  - move => t1 ? t2 ? c c' ?; f_equal; auto.
-  - by move => ty t' IH c c' ?; rewrite -addnS IH.
+  - move => n c c' H; elimif_omega.
+  - move => tl IHtl tr IHtr c c' H; f_equal; auto.
+  - by move => ty t' IH c c' H; rewrite -addnS IH.
   - by move => t IH ty c c' H; rewrite IH.
   - by move => t IH c c' H; rewrite IH.
 Qed.
 
 Lemma subst_shift_distr :
-  forall n d c ts t,
-  shift_term d (n + c) (subst_term n ts t) =
-  subst_term n (map (shift_term d c) ts) (shift_term d (size ts + n + c) t).
+  forall n m d c ts t,
+  shift_term d (n + c) (subst_term n m ts t) =
+  subst_term n m (map (shift_term d c) ts) (shift_term d (size ts + n + c) t).
 Proof.
-  move => n d c ts t; elim: t n => /=; try congruence.
-  - move => m n; rewrite /subst_termv size_map; elimif_omega.
-    - rewrite !nth_default ?size_map /=; try ssromega.
-      rewrite (subnAC _ n) subnK; elimif_omega.
-    - rewrite -shift_shift_distr // nth_map' /=.
-      f_equal; apply nth_equal; rewrite size_map; elimif_omega.
-  - by move => ty t IH n; rewrite (IH n.+1) addnS addSn.
+  move => n m d c ts t; elim: t n m => /=; try (move: addnS addSn; congruence).
+  move => v n m; rewrite /subst_termv size_map; elimif_omega.
+  - rewrite shift_typemap_distr !nth_default ?size_map /=; try ssromega.
+    rewrite (subnAC _ n) subnK; elimif_omega.
+  - rewrite shift_typemap_distr -shift_shift_distr // nth_map' /=.
+    do 2 f_equal; apply nth_equal; rewrite size_map; elimif_omega.
 Qed.
 
 Lemma shift_subst_distr :
-  forall n d c t ts, c <= n ->
-  shift_term d c (subst_term n ts t) = subst_term (d + n) ts (shift_term d c t).
+  forall n m d c ts t, c <= n ->
+  shift_term d c (subst_term n m ts t) =
+  subst_term (d + n) m ts (shift_term d c t).
 Proof.
-  move => n d c t ts; elim: t n c => /=.
-  - move => n m c H; elimif_omega.
-    by rewrite /subst_termv shift_add ?addn0 // (addnC n) subnDl.
-  - move => tl IHl tr IHr n c H; f_equal; auto.
-  - move => ty t IH n c H; f_equal; rewrite -addnS IH //.
-  - by move => t IH ty n c H; rewrite IH.
-  - by move => t IH n c H; rewrite IH.
+  move => n m d c ts t; elim: t n m c => /=.
+  - move => v n m c H; elimif_omega.
+    by rewrite /subst_termv shift_typemap_distr
+      shift_add ?addn0 // (addnC v) subnDl.
+  - move => tl IHl tr IHr n m c H; f_equal; auto.
+  - move => ty t IH n m c H; f_equal; rewrite -addnS IH //.
+  - by move => t IH ty n m c H; rewrite IH.
+  - by move => t IH n m c H; rewrite IH.
 Qed.
 
 Lemma subst_shift_cancel :
-  forall n d c t ts, n <= d ->
-  subst_term (c + n) ts (shift_term (size ts + d) c t) = shift_term d c t.
+  forall n m d c ts t, c <= n -> size ts <= d -> n - c <= d - size ts ->
+  subst_term n m ts (shift_term d c t) = shift_term (d - size ts) c t.
 Proof.
-  move => n d c t ts; elim: t c => /=.
-  - move => v c H; elimif_omega.
+  move => n m d c ts t; elim: t n m c => /=.
+  - move => v n m c H H0 H1; elimif_omega.
     rewrite /subst_termv nth_default /=; f_equal; ssromega.
-  - by move => tl IHtl tr IHtr c H; rewrite IHtl // IHtr.
-  - by move => ty t IH c H; rewrite -addSn IH.
-  - by move => t IH ty c H; rewrite IH.
-  - by move => t IH c H; rewrite IH.
+  - by move => tl IHtl tr IHtr n m c H H0 H1; rewrite IHtl // IHtr.
+  - by move => ty t IH n m c H H0 H1; rewrite IH.
+  - by move => t IH ty n m c H H0 H1; rewrite IH.
+  - by move => t IH n m c H H0 H1; rewrite IH.
 Qed.
 
 Lemma subst_subst_distr :
-  forall n m t xs ys,
-  subst_term (m + n) xs (subst_term m ys t) =
-  subst_term m (map (subst_term n xs) ys) (subst_term (size ys + m + n) xs t).
+  forall n n' m m' xs ys t,
+  subst_term (n' + n) (m' + m) xs (subst_term n' m' ys t) =
+  subst_term n' m' (map (subst_term n m xs) ys)
+    (subst_term (size ys + n' + n) (m' + m) xs t).
 Proof.
-  move => n m t; elim: t m => /=; try congruence.
-  - move => v m xs ys; elimif_omega; rewrite /subst_termv.
-    - rewrite -{5}(add0n m) -addnA -{2}(size_map (subst_term n xs) ys)
-        subst_shift_cancel; last apply leq_addr.
-      rewrite nth_default /=; last ssromega.
-      rewrite /subst_termv subnAC subnK ?subnDA; elimif_omega.
-    - rewrite -shift_subst_distr // size_map nth_map'; f_equal.
-      apply nth_equal; rewrite size_map /=; elimif_omega.
-  - by move => ty t IH m xs ys; rewrite -addSn IH addnS addSn.
+  move => n n' m m' xs ys t; elim: t n' m' => /=;
+    try (move: addSn addnS; congruence).
+  move => v n' m'; elimif_omega; rewrite /subst_termv.
+  - rewrite -!shift_typemap_distr (subst_shift_cancel n') // size_map
+      ?subn0 -?addnA ?addKn ?leq_addr // nth_default /=; last ssromega.
+    rewrite /subst_termv subnAC subnK /subnDA; last ssromega.
+    rewrite shift_typemap_distr !subnDA; elimif_omega.
+  - rewrite -!shift_typemap_distr -shift_subst_distr //
+      subst_shifttyp_distr // (nth_map' (subst_term _ _ _)) /= /subst_termv.
+    do 2 f_equal; apply nth_equal.
+    rewrite size_map; elimif_omega.
 Qed.
 
 Lemma subst_app :
-  forall n t xs ys,
-  subst_term n xs (subst_term (size xs + n) ys t) = subst_term n (xs ++ ys) t.
+  forall n m xs ys t,
+  subst_term n m xs (subst_term (size xs + n) m ys t) =
+  subst_term n m (xs ++ ys) t.
 Proof.
-  move => n t xs ys; elim: t n => /=; try congruence.
-  - move => v n; elimif_omega; rewrite /subst_termv.
-    - rewrite -{1}(add0n n) subst_shift_cancel //
-        nth_cat size_cat !subnDA (subnAC _ (size xs)); f_equal; elimif_omega.
-    - rewrite nth_cat; f_equal; elimif_omega; apply nth_equal; ssromega.
-  - by move => ty t IH n; rewrite -addnS IH.
+  move => n m xs ys t; elim: t n m => /=; try (move: addnS; congruence).
+  move => v n m; elimif_omega; rewrite /subst_termv.
+  - rewrite -!shift_typemap_distr subst_shift_cancel //
+      ?leq_addr ?subn0 ?addKn // nth_cat size_cat !subnDA (subnAC _ (size xs)).
+    f_equal; elimif_omega.
+  - rewrite nth_cat; do 2 f_equal; elimif_omega; apply nth_equal; ssromega.
 Qed.
 
-Lemma subst_nil : forall n t, subst_term n [::] t = t.
+Lemma subst_nil : forall n m t, subst_term n m [::] t = t.
 Proof.
-  move => n t; elim: t n => /=; try congruence.
-  move => v n; rewrite /subst_termv nth_nil /= -fun_if; elimif_omega.
+  move => n m t; elim: t n m => /=; try congruence.
+  move => v n m; rewrite /subst_termv nth_nil /= -fun_if; elimif_omega.
 Qed.
+
+Lemma redappl :
+  forall t1 t1' t2, t1 ->r t1' -> app t1 t2 ->r app t1' t2.
+Proof.
+  move => t1 t1' t2; elim => // {t1 t1'} t1 t1' t1'' H H0 H1.
+  by apply rt1n_trans with (app t1' t2) => //; constructor.
+Qed.
+
+Lemma redappr :
+  forall t1 t2 t2', t2 ->r t2' -> app t1 t2 ->r app t1 t2'.
+Proof.
+  move => t1 t2 t2'; elim => // {t2 t2'} t2 t2' t2'' H H0 H1.
+  by apply rt1n_trans with (app t1 t2') => //; constructor.
+Qed.
+
+Lemma redabs : forall ty t t', t ->r t' -> abs ty t ->r abs ty t'.
+Proof.
+  move => ty t t'; elim => // {t t'} t t' t'' H H0 H1.
+  by apply rt1n_trans with (abs ty t') => //; constructor.
+Qed.
+
+Lemma reduapp : forall t t' ty, t ->r t' -> uapp t ty ->r uapp t' ty.
+Proof.
+  move => t t' ty; elim => // {t t'} t t' t'' H H0 H1.
+  by apply rt1n_trans with (uapp t' ty) => //; constructor.
+Qed.
+
+Lemma reduabs : forall t t', t ->r t' -> uabs t ->r uabs t'.
+Proof.
+  move => t t'; elim => // {t t'} t t' t'' H H0 H1.
+  by apply rt1n_trans with (uabs t') => //; constructor.
+Qed.
+
+Hint Resolve redappl redappr redabs reduapp reduabs.
+
+Module confluence_proof.
+
+Reserved Notation "t ->rp t'" (at level 70, no associativity).
+
+Inductive parred : relation term :=
+  | parredfst  : forall ty t1 t1' t2 t2', t1 ->rp t1' -> t2 ->rp t2' ->
+                 app (abs ty t1) t2 ->rp subst_term 0 0 [:: t2'] t1'
+  | parredsnd  : forall t t' ty, t ->rp t' ->
+                 uapp (uabs t) ty ->rp typemap (subst_typ^~ [:: ty]) 0 t'
+  | parredvar  : forall n, var n ->rp var n
+  | parredapp  : forall t1 t1' t2 t2',
+                 t1 ->rp t1' -> t2 ->rp t2' -> app t1 t2 ->rp app t1' t2'
+  | parredabs  : forall ty t t', t ->rp t' -> abs ty t ->rp abs ty t'
+  | parreduapp : forall t t' ty, t ->rp t' -> uapp t ty ->rp uapp t' ty
+  | parreduabs : forall t t', t ->rp t' -> uabs t ->rp uabs t'
+  where "t ->rp t'" := (parred t t').
+
+Fixpoint reduce_all_redex t : term :=
+  match t with
+    | var _ => t
+    | app (abs ty t1) t2 =>
+      subst_term 0 0 [:: reduce_all_redex t2] (reduce_all_redex t1)
+    | app t1 t2 => app (reduce_all_redex t1) (reduce_all_redex t2)
+    | abs ty t' => abs ty (reduce_all_redex t')
+    | uapp (uabs t) ty =>
+      typemap (subst_typ^~ [:: ty]) 0 (reduce_all_redex t)
+    | uapp t ty => uapp (reduce_all_redex t) ty
+    | uabs t => uabs (reduce_all_redex t)
+  end.
+
+Lemma parred_refl : forall t, parred t t.
+Proof.
+  by elim; constructor.
+Qed.
+
+Hint Resolve parred_refl.
+
+Lemma betared1_in_parred : inclusion reduction1 parred.
+Proof.
+  by apply reduction1_ind; constructor.
+Qed.
+
+Lemma parred_in_betared : inclusion parred reduction.
+Proof.
+  apply parred_ind => //; auto.
+  - move => ty t1 t1' t2 t2' H H0 H1 H2.
+    apply rtc_trans' with (app (abs ty t1') t2); auto.
+    apply rtc_trans' with (app (abs ty t1') t2'); auto.
+    apply rtc_step; constructor.
+  - move => t t' ty H H0.
+    apply rtc_trans' with (uapp (uabs t') ty); auto.
+    apply rtc_step; constructor.
+  - move => t1 t1' t2 t2' H H0 H1 H2; apply rtc_trans' with (app t1 t2'); auto.
+Qed.
+
+Lemma shift_parred :
+  forall t t' d c, t ->rp t' -> shift_term d c t ->rp shift_term d c t'.
+Proof.
+  move => t t' d c H; move: t t' H d c.
+  refine (parred_ind _ _ _ _ _ _ _ _) => //=; try by constructor.
+  - move => ty t1 t1' t2 t2' H H0 H1 H2 d c.
+    rewrite (subst_shift_distr 0).
+    by constructor.
+  - move => t t' ty H H0 d c.
+    rewrite shift_typemap_distr.
+    by constructor.
+Qed.
+
+Lemma shifttyp_parred :
+  forall t t' d c,
+  t ->rp t' -> typemap (shift_typ d) c t ->rp typemap (shift_typ d) c t'.
+Proof.
+  move => t t' d c H; move: t t' H d c.
+  refine (parred_ind _ _ _ _ _ _ _ _) => /=; try constructor; auto.
+  - move => ty t1 t1' t2 t2' H H0 H1 H2 d c.
+    by rewrite (shifttyp_subst_distr d c 0 0) add0n /=; constructor.
+  - move => t t' ty H H0 n m.
+    by rewrite -{3}(add0n m) substtyp_shifttyp_distr /= 2!add1n; constructor.
+Qed.
+
+Lemma substtyp_parred :
+  forall n tys t t', t ->rp t' ->
+  typemap (subst_typ^~ tys) n t ->rp typemap (subst_typ^~ tys) n t'.
+Proof.
+  move => n tys t t' H; move: t t' H n.
+  refine (parred_ind _ _ _ _ _ _ _ _) => /=; try constructor; auto.
+  - move => ty t1 t1' t2 t2' H H0 H1 H2 n.
+    by rewrite substtyp_subst_distr // subn0; constructor.
+  - move => t t' ty H H0 n.
+    by rewrite -{3}(add0n n) substtyp_substtyp_distr /= 2!add1n; constructor.
+Qed.
+
+Lemma subst_parred :
+  forall n m ps t t', Forall (prod_curry parred) ps -> t ->rp t' ->
+  subst_term n m [seq fst p | p <- ps] t ->rp
+  subst_term n m [seq snd p | p <- ps] t'.
+Proof.
+  move => n m ps t t' H H0; move: t t' H0 n m.
+  refine (parred_ind _ _ _ _ _ _ _ _) => /=; try constructor; auto.
+  - move => ty tl tl' tr tr' H0 H1 H2 H3 n m.
+    by rewrite (subst_subst_distr n 0 m 0) /= 2!add1n add0n; constructor.
+  - by move => t t' ty H0 H1 n m; rewrite subst_substtyp_distr //=; constructor.
+  - move => v n m.
+    rewrite /subst_termv !size_map.
+    case: ifP => // _.
+    elim: ps H (v - n) => //= {v} [[t t']] ts IH [H H0] [| v] //=.
+    - by apply shifttyp_parred, shift_parred.
+    - by rewrite subSS; apply IH.
+Qed.
+
+Lemma parred_all_lemma : forall t t', t ->rp t' -> t' ->rp reduce_all_redex t.
+Proof with auto.
+  fix 3 => t t' H; inversion H; subst => {H} /=; try by constructor; auto.
+  - apply (subst_parred 0 0 [:: (t2', reduce_all_redex t2)]) => /=; auto.
+  - by apply substtyp_parred; apply parred_all_lemma.
+  - destruct t1; try by constructor; auto.
+    by inversion H0; constructor; auto.
+  - destruct t0; try by constructor; auto.
+    by inversion H0; constructor; auto.
+Qed.
+
+Lemma parred_confluent : confluent parred.
+Proof.
+  by move => t1 t2 t3 H H0;
+    exists (reduce_all_redex t1); split; apply parred_all_lemma.
+Qed.
+
+Theorem betared_confluent : confluent reduction.
+Proof.
+  apply (rtc_confluent' parred
+    betared1_in_parred parred_in_betared parred_confluent).
+Qed.
+
+End confluence_proof.
